Use new naming, functions

src/code.lean
@@ -3,7 +3,16 @@ import computability.encoding
 import pair
 import part
 
-open computability (encode_nat decode_nat)
+namespace num
+
+@[simp] lemma bit1_ne_zero (n : num) : n.bit1 ≠ 0 := by cases n; trivial
+@[simp] lemma bit0_zero_iff_zero (n : num) : n.bit0 = 0 ↔ n = 0 :=
+⟨λ h, by { cases n, { refl, }, contradiction, }, by { rintro rfl, refl, }⟩
+@[simp] lemma succ_ne_zero (n : num) : n + 1 ≠ 0 := by cases n; trivial
+
+end num
+
+open num (to_bits of_bits)
 
 section
 parameter (ι : Type)
@@ -34,10 +43,10 @@ parameter {ι}
 | (code.bit b) := nat.bit b
 | (code.pair f g) := λ v, do x ← f.eval v, y ← g.eval v, return (nat.mkpair' x y) 
 | (code.comp f g) := λ v, g.eval v >>= f.eval
-| (code.case f g h) := λ v, match encode_nat v with
+| (code.case f g h) := λ v, match to_bits v with
   | [] := h.eval 0
-  | (ff :: xs) := f.eval (decode_nat xs)
-  | (tt :: xs) := g.eval (decode_nat xs)
+  | (ff :: xs) := f.eval (of_bits xs)
+  | (tt :: xs) := g.eval (of_bits xs)
 end
 | (code.fix f) := pfun.fix $ λ v, (f.eval v).map $ λ v',
   if (nat.unpair' v').1 = 0 then sum.inl (nat.unpair' v').2 else sum.inr (nat.unpair' v').2
@@ -69,14 +78,19 @@ by simp [code.id, nat.bit, ← nat.mkpair'_zero]
 def append_const : list bool → code
 | [] := code.id
 | (b :: bs) := bit b ∘ (append_const bs)
-lemma append_const_apply (bs : list bool) (n : ℕ) :
-  (append_const bs).eval n = part.some (bs.foldr nat.bit n) :=
-by { induction bs with _ _ ih, { simp [append_const], }, simp [append_const, ih], }
-lemma append_const_apply' (bs : list bool) (n : ℕ) (hn : n ≠ 0 ∨ bs.last'.get_or_else tt = tt) :
-  (append_const bs).eval n = part.some (decode_nat (bs ++ encode_nat n)) :=
-by { cases hn, rw [append_const_apply, computability.append_bits _ hn], rw [append_const_apply, computability.append_bits' _ hn], }
+lemma append_const_apply' (bs : list bool) (n : ℕ) (hn : n ≠ 0 ∨ bs ∈ set.range to_bits) :
+  (append_const bs).eval n = part.some (of_bits (bs ++ to_bits n)) :=
+begin
+  induction bs with hd tl ih, { simp [append_const], },
+  specialize ih _, { cases hn, { tauto, }, exact or.inr (num.mem_to_bits_range_of_cons hn), },
+  by_cases tl = [],
+  { subst h, simp [num.mem_to_bits_range_iff] at hn,
+    cases hn, swap, { subst hn, simp [append_const], refl, },
+    cases hd; simp [append_const, ih, (show (to_bits n) ≠ [], by simpa)]; refl, },
+  cases hd; simp [append_const, ih, h]; refl,
+end
 
-protected def code.const (c : ℕ) : code := (append_const (encode_nat c)) ∘ zero
+protected def code.const (c : ℕ) : code := (append_const (to_bits c)) ∘ zero
 @[simp] lemma const_apply (c n : ℕ) : (code.const c).eval n = part.some c :=
 begin
   simp only [code.const, code.eval, zero_apply, part.bind_eq_bind, part.bind_some],
@@ -88,9 +102,9 @@ end
 def to_bit : code := case one one zero
 @[simp] lemma to_bit_apply (n : ℕ) : to_bit.eval n = part.some (if n = 0 then 0 else 1) :=
 begin
-  have := computability.encode_nat_nil_iff_zero n,
+  have : to_bits n = [] ↔ n = 0 := by simp,
   simp only [to_bit, code.eval],
-  rcases (encode_nat n) with _|_|_,
+  rcases (to_bits n) with _|_|_,
   all_goals { intro, simp * at *, },
 end
 
@@ -100,8 +114,9 @@ def tail : code := snd ∘ (bit ff) ∘ (bit tt) ∘ (bit tt)
 by simp [tail, nat.bit, ← nat.mkpair'_one]
 @[simp] lemma tail_apply_bit0 (n : ℕ) : tail.eval (bit0 n) = part.some n :=
 begin
-  cases n;
-  simp [tail, nat.bit, nat.unpair', list.unpair, list.unpair', list.take_while, list.after],
+  cases n, { simp [tail], dec_trivial, },
+  simp [tail, nat.unpair', nat.bit, num.bit0_of_bit0, num.bit1_of_bit1, nat.unpair',
+    list.unpair, list.unpair', list.take_while, list.after],
 end
 
 /-- Evaluates `f` and `g` on the input;, then appends the bit `to_bit f` to `g` -/
@@ -114,7 +129,7 @@ begin
   cases (g.eval n) with d₂ v₂, by_cases h₂ : d₂, swap, { simp [h₂], }, simp only [h₂, part.mk_some],
   cases v₁ h₁,
   { simp [nat.mkpair'_zero, nat.bit], },
-  { simp [nat.mkpair'_one, nat.bit], }
+  { simp [nat.mkpair'_one, nat.bit, num.bit0_of_bit0, num.bit1_of_bit1], }
 end
 
 protected def code.ite (c f g : code) : code :=
