src/lists.lean
@@ -1,23 +1,39 @@
 import tactic
 
 namespace list
-/- These are just a few misc lemmas (might already be in mathlib even)
-  about lists -/
+variables {α : Type*}
+
+@[simp] theorem append_inj'_iff (s₁ s₂ : list α) {t₁ t₂ : list α} (hl : length t₁ = length t₂) :
+  s₁ ++ t₁ = s₂ ++ t₂ ↔ s₁ = s₂ ∧ t₁ = t₂ :=
+⟨λ h, append_inj' h hl, by cc⟩
+
+
+@[simp] theorem init_nil : (@list.nil α).init = [] := rfl
+
+@[simp] theorem init_singleton (x : α) : [x].init = [] := rfl
+
+
+@[simp] lemma last'_reverse {α : Type*} (xs : list α) : xs.reverse.last' = xs.head' :=
+by cases xs; simp
+
+lemma last'_eq_head'_reverse {α : Type*} (xs : list α) : xs.last' = xs.reverse.head' :=
+by simpa using xs.reverse.last'_reverse
+
+/-- Take cases on the last element of the list. Like `reverse_rec_on`, this can be used
+for constructing data as well. -/
+def reverse_cases_on {α : Type*} {C : list α → Sort*} (l : list α) (h₀ : C [])
+  (case : ∀ st lt, C (st ++ [lt])) : C l :=
+by { induction l using list.reverse_rec_on, { exact h₀, }, { apply case, } }
+
+/-! ### after -/
+section after
 
 lemma after_spec {α : Type*} (p : α → Prop) [decidable_pred p]
-  (as : list α) (x : α) (xs : list α) (has : ∀ a ∈ as, ¬ p a) (hx : p x) :
+  (as : list α) (x : α) (xs : list α) (has : ∀ a ∈ as, ¬p a) (hx : p x) :
   (as ++ x :: xs).after p = xs :=
 begin
-  induction as with hd tl ih, { simp [list.after, hx], },
-  simp [list.after, has hd, ih (λ a ha, has a (or.inr ha))],
-end
-
-lemma take_while_spec {α : Type*} (p : α → Prop) [decidable_pred p]
-  (as : list α) (x : α) (xs : list α) (has : ∀ a ∈ as, p a) (hx : ¬ p x) :
-  (as ++ x :: xs).take_while p = as :=
-begin
-  induction as with hd tl ih, { simp [list.take_while, hx], },
-  simp [list.take_while, has hd, ih (λ a ha, has a (or.inr ha))],
+  induction as with hd tl ih, { simp [after, hx], },
+  simp [after, has hd, ih (λ a ha, has a (or.inr ha))],
 end
 
 lemma after_sublist {α : Type*} (p : α → Prop) [decidable_pred p] (xs : list α) :
@@ -33,71 +49,25 @@ by { simp only [after], split_ifs, { refl, }, { apply after_sublist, } }
 
 lemma after_length_lt {α : Type*} (p : α → Prop) [decidable_pred p] {xs : list α} :
   (xs.after p).length < xs.length ↔ 0 < xs.length :=
-begin
-  split, { exact pos_of_gt, },
+⟨pos_of_gt, begin
   cases xs, { simp, },
-  exact (λ _, nat.lt_succ_iff.mpr (length_le_of_sublist (after_sublist_strict _ _ _))),
-end
+  intro, simpa [nat.lt_succ_iff] using length_le_of_sublist (after_sublist_strict p _ _),
+end⟩
 
-lemma empty_ff_iff_neq_nil {α : Type*} {ls : list α} : ls.empty = ff ↔ ls ≠ [] :=
-by { convert not_congr (@empty_iff_eq_nil _ ls), simp, }
 
-@[simp] lemma append_singleton' {α : Type*} (x : α) : append [x] = cons x :=
-by { ext : 1, simp, }
+end after
 
-/-- Really annoying, I couldn't get the standard `cases_on` types to work -/
-@[simp] def cases_on' {α β : Type*} (ls : list α) (start : β) (step : α → list α → β) : β :=
-@list.cases_on _ (λ _, β) ls start step
+/-! ### take_while -/
+section take_while
 
-@[simp] lemma foldl_of_cons {α : Type*} (ls : list α) :
-  ls.foldl (flip list.cons) [] = ls.reverse :=
+lemma take_while_spec {α : Type*} (p : α → Prop) [decidable_pred p]
+  (as : list α) (x : α) (xs : list α) (has : ∀ a ∈ as, p a) (hx : ¬ p x) :
+  (as ++ x :: xs).take_while p = as :=
 begin
-  suffices : ∀ b, ls.foldl (flip list.cons) b = ls.reverse ++ b,
-  { simpa using this [], },
-  induction ls with hd tl ih, { simp, },
-  intro b, simp [ih], refl,
+  induction as with hd tl ih, { simp [take_while, hx], },
+  simp [take_while, has hd, ih (λ a ha, has a (or.inr ha))],
 end
 
-@[simp] lemma last_eq_none_iff {α : Type*} (ls : list α) :
-  ls.last' = none ↔ ls = [] :=
-begin
-  split, swap, { intro h, rw h, refl, },
-  contrapose, induction ls with hd tl ih, { simp, },
-  intro, cases tl, { simp, }, simpa using ih,
-end
-
-@[simp] lemma last'_cons {α : Type*} (hd : α) (tl : list α) (ht : tl ≠ []) :
-  (hd :: tl).last' = tl.last' :=
-by { induction tl, { cases ht rfl, }, simp, }
-
-lemma last'_of_tail {α : Type*} {l : list α} {x : α} (hx : x ∈ l.tail.last') : x ∈ l.last' :=
-by { cases l with hd tl, { simp at hx, contradiction, }, cases tl, { simp at hx, contradiction, }, simpa using hx, } 
-
-lemma last_cons_is_some {α : Type*} (hd : α) (tl : list α) :
-  (hd :: tl).last'.is_some := by induction tl; simp [*]
-
-@[simp] lemma drop_last {α : Type*} (ls : list α) (n : ℕ) (hn : n < ls.length) :
-  (ls.drop n).last' = ls.last' :=
-begin
-  induction ls with hd tl ih generalizing n, { simp, },
-  cases n, { simp, },
-  specialize ih n _, { simpa [nat.succ_eq_add_one] using hn, },
-  have : tl ≠ [], { intro h, subst h, simpa using hn, },
-  simp [this, ih],
-end
-
-example {α: Type} (hd : α) (tl : list α) (x : α) (hx : x ∈ tl.last') : x ∈ (hd :: tl).last' := mem_last'_cons hx
-
-lemma after_last {α : Type*} (ls : list α) (p : α → Prop) [decidable_pred p] :
-  ∀ x ∈ (ls.after p).last', x ∈ ls.last' :=
-begin
-  induction ls with hd tl ih, { simp [after], },
-  intros x hx,
-  by_cases h : p hd,
-  { simp [h, after, ← option.mem_def] at ⊢ hx, apply mem_last'_cons hx, },
-  specialize ih x _,
-  { simp [h, after] at hx, exact hx, },
-  apply mem_last'_cons ih,
-end
+end take_while
 
 end list
