src/pair.lean
@@ -1,341 +1,109 @@
-import data.num.basic
-import data.nat.log
-import computability.encoding
+/-
+Copyright (c) 2022 Praneeth Kolichala. All rights reserved.
+Released under Apache 2.0 license as described in the file LICENSE.
+Authors: Praneeth Kolichala
+-/
+-- import data.num.to_bits
+import to_bits
+import data.list.basic
 import lists
 
-attribute [simp] computability.decode_encode_nat
-attribute [simp] nat.log_mul_base
+/-!
+# Efficient Pairing
 
-namespace nat
+One issue with the standard `nat.mkpair` is that it isn't suitable for polytime encoding.
+While the pairing function itself runs in polynomial time, repeated applications of it
+(even only polynomially many) can cause the result to blow up exponentially. Therefore, we cannot
+e.g. create lists by encoding `[a, b, c, ...] = (a, (b, (c, ...)))` in polynomial time.
 
-@[simp] lemma log_base_mul (b n : ℕ) (hb : 1 < b) (hn : 0 < n) : log b (b * n) = (log b n) + 1 :=
-by { rw mul_comm, exact nat.log_mul_base b n hb hn, } 
+This file defines an efficient pairing function. We first define a pairing function
+on lists which take `list bool`'s of `a` and `b`, and outputs an encoding of `(a, b)`,
+which has size `a.length + b.length + O(log a.length)` (so only logarithmic overhead in the first
+argument). We then extend this to `nat`'s using `encode_num`.
 
-@[simp] lemma log_base_mul_add (b n x : ℕ) (hb : 1 < b) (hn : 0 < n) (hx : x < b) : log b (b * n + x) = (log b n) + 1 :=
-begin
-  suffices : log b ((b * n + x) / b * b) = log b n + 1, { simpa, },
-  conv_lhs { rw [add_comm, add_mul_div_left _ _ (nat.zero_lt_one.trans hb), div_eq_of_lt hx], },
-  simp [hb, hn],
-end
+## Main definitions
 
-@[simp] lemma log2_bit (n : ℕ) (hn : 0 < n) (b : bool) : log 2 (bit b n) = (log 2 n) + 1 :=
-begin
-  cases n, { simp at hn, contradiction, },
-  cases b; simp [nat.bit, nat.bit0_val n.succ, nat.bit1_val n.succ],
-end
+### List pairing
+  - `list.mkpair'` - Encodes a pair of `list bool`'s with linear overhead i.e.
+      `|(a, b)| = O(|a|) + |b|`, where `|a|` denotes the size of list `a`.
+  - `list.mkpair` - Encodes a pair of `list bool`'s with logarithmic overhead i.e.
+      `|(a, b)| = |a| + |b| + O(log |a|)`
 
-end nat
-
-open computability (encode_nat decode_nat)
-
-namespace option
-
-lemma iget_eq_get_of_some {α : Type*} [inhabited α] (x : option α) (h : x.is_some) :
-  x.iget = get h := by { cases x, { cases h, }, refl, }
-
-
-lemma get_or_else_eq_get_of_some {α : Type*} {x : option α} (d : α) (h : x.is_some) :
-  x.get_or_else d = get h := by { cases x, { cases h, }, refl, }
-
-lemma is_some_iff_not_is_none {α : Type*} (x : option α) :
-  x.is_some ↔ ¬x.is_none := by cases x; simp
-
-lemma get_or_else_of_mem {α : Type*} {x : option α} {y : α} (hy : y ∈ x) (d : α) :
-  x.get_or_else d = y := by { cases x, { cases hy, }, simpa using hy, }
-
-end option
-
-namespace pos_num
-
-lemma bit0_val (n : pos_num) : (bit0 n : ℕ) = 2 * (n : ℕ) :=
-by { rw cast_bit0 n, exact nat.bit0_val _, }
-
-lemma bit1_val (n : pos_num) : (bit1 n : ℕ) = 2 * (n : ℕ) + 1 :=
-by { rw cast_bit1 n, exact nat.bit1_val _, }
-
-end pos_num
-
-namespace computability
-
-
-lemma encode_decode_pos_num {ls : list bool} (h : ls.last'.iget = tt) :
-  encode_pos_num (decode_pos_num ls) = ls :=
-begin
-  induction ls with hd tl ih, { exfalso, simpa using h, },
-  cases tl with h t, { simp at h, subst h, refl, },
-  specialize ih _, { simpa using h, },
-  cases hd; simp [decode_pos_num, encode_pos_num, ih],
-end
-
-lemma encode_decode_num {ls : list bool} (h : ls.last'.get_or_else tt = tt) :
-  encode_num (decode_num ls) = ls :=
-begin
-  cases ls with hd tl, { refl, },
-  simp only [decode_num], simp only [encode_num, if_false, pos_num.cast_to_num],
-  apply encode_decode_pos_num, convert h,
-  rwa [option.iget_eq_get_of_some, option.get_or_else_eq_get_of_some],
-  apply list.last_cons_is_some,
-end
-
-lemma encode_decode_nat (ls : list bool) (h : ls.last'.get_or_else tt = tt) :
-  encode_nat (decode_nat ls) = ls :=
-by simp [encode_nat, decode_nat, encode_decode_num h]
-
-lemma encode_pos_num_last (n : pos_num) : tt ∈ (encode_pos_num n).last' :=
-begin
-  induction n with b₀ ih b₀ ih, { simp, refl, },
-  all_goals { simp only [encode_pos_num], cases encode_pos_num b₀, { cases ih, }, simp [ih], },
-end
-
-lemma encode_num_bit0 (n : num) (hn : n ≠ 0): encode_num (bit0 n) = ff :: encode_num n :=
-begin
-  cases n, { contradiction, },
-  change bit0 (num.pos n) with num.pos (bit0 n),
-  simp [encode_num, encode_pos_num, pos_num.bit0_of_bit0],
-end
-
-@[simp] lemma encode_nat_bit0 (n : ℕ) (hn : n ≠ 0) : encode_nat (bit0 n) = ff :: encode_nat n :=
-by simp [encode_nat, encode_num_bit0, hn]
-
-@[simp] lemma encode_num_bit1 (n : num) : encode_num (bit1 n) = tt :: encode_num n :=
-begin
-  cases n, { refl, },
-  change bit1 (num.pos n) with num.pos (bit1 n),
-  simp [encode_num, encode_pos_num, pos_num.bit1_of_bit1],
-end
-
-@[simp] lemma encode_nat_bit1 (n : ℕ) : encode_nat (bit1 n) = tt :: encode_nat n :=
-by simp [encode_nat, encode_num_bit1]
-
-@[simp] lemma decode_nat_bit (b : bool) (bs : list bool) (hbs : bs ≠ []) : decode_nat (b :: bs) = nat.bit b (decode_nat bs) :=
-by cases b; simp [decode_nat, decode_num]; simp [decode_pos_num, hbs, nat.bit]
-
-@[simp] lemma decode_nat_bit1 (bs : list bool) : decode_nat (tt :: bs) = bit1 (decode_nat bs) :=
-by { cases bs, { refl, }, simp [nat.bit], }
-
-lemma decode_nat_invalid (bs : list bool) (h : ff ∈ bs.last') : decode_nat bs = decode_nat (bs ++ [tt]) :=
-begin
-  induction bs with hd tl ih, { simp at h, contradiction, },
-  cases tl with h t,
-  { simp at h, subst h, dec_trivial, },
-  specialize ih _, { rw option.mem_iff, simpa using h, },
-  cases hd; simp [ih],
-end
-
-lemma encode_num_last (n : num) : (encode_num n).last'.get_or_else tt = tt :=
-by { cases n, { refl, }, apply option.get_or_else_of_mem (encode_pos_num_last n), }
-
-@[simp] lemma encode_nat_last (n : ℕ) : (encode_nat n).last'.get_or_else tt = tt := encode_num_last n
-
-@[simp] lemma encode_pos_num_len (n : pos_num) : (encode_pos_num n).length = (nat.log 2 n) + 1 :=
-begin
-  induction n, { simp [encode_pos_num], },
-  { simpa [encode_pos_num, pos_num.bit1_val], },
-  { simpa [encode_pos_num, pos_num.bit0_val], },
-end
-
-lemma encode_num_len (n : num) : (encode_num n).length = if n = 0 then 0 else (nat.log 2 n) + 1 :=
-begin
-  cases n, { refl, },
-  have : num.pos n ≠ 0 := dec_trivial,
-  simp [encode_nat, encode_num, this],
-end
-
-lemma encode_nat_len (n : ℕ) : (encode_nat n).length = if n = 0 then 0 else nat.log 2 n + 1 :=
-by simp [encode_nat, encode_num_len n]
-
-lemma encode_nat_len_le (n : ℕ) : (encode_nat n).length ≤ nat.log 2 n + 1 :=
-by { rw encode_nat_len, split_ifs; simp, }
-
-@[simp] lemma encode_nat_zero : encode_nat 0 = [] := rfl
-@[simp] lemma encode_nat_one : encode_nat 1 = [tt] := rfl
-@[simp] lemma decode_nat_nil : decode_nat [] = 0 := rfl
-
-lemma encode_nat_succ_ne_nil (n : ℕ) : encode_nat n.succ ≠ [] :=
-by simp [← list.length_eq_zero, encode_nat_len]
-
-lemma encode_nat_nil_iff_zero (n : ℕ) : encode_nat n = [] ↔ n = 0 :=
-⟨λ h, by { cases n, refl, cases encode_nat_succ_ne_nil n h, }, λ h, by { rw h, refl, }⟩
-
-lemma append_bits {n : ℕ} (bs : list bool) (h : n ≠ 0) : decode_nat (bs ++ encode_nat n) = bs.foldr nat.bit n :=
-begin
-  induction bs with hd tl ih, { simp, },
-  cases n, { contradiction, },
-  rw [list.cons_append, decode_nat_bit], { simp [ih] },
-  exact list.append_ne_nil_of_ne_nil_right _ _ (encode_nat_succ_ne_nil n),
-end
-
-lemma append_bits' (n : ℕ) {bs : list bool} (h : bs.last'.get_or_else tt = tt) : decode_nat (bs ++ encode_nat n) = bs.foldr nat.bit n :=
-begin
-  induction bs with hd tl ih, { simp, },
-  cases tl with h t,
-  { simp at h, subst h, simp [nat.bit], },
-  rw list.last'_cons at h,
-  { specialize ih h, simp only [list.cons_append] at ih, simp [ih], },
-  trivial,
-end
-
-lemma decode_nat_lb (l : list bool) (h : l.last'.get_or_else tt = tt) : (decode_nat l : ℤ) ≤ (2^l.length : ℤ) - 1 :=
-begin
-  induction l with hd tl ih, { simp, },
-  cases hd,
-  { have : tl ≠ [], { intro H, simp [H] at h, contradiction, },
-    specialize ih _, { simp [this] at h, assumption, },
-    simp only [this, nat.bit, decode_nat_bit, not_false_iff, ne.def, bool.cond_ff, list.length, pow_succ],
-    rw nat.bit0_val, simp, linarith [ih], },
-  specialize ih _,
-  { cases tl, { refl }, simpa using h, },
-  simp only [list.length, decode_nat_bit1, pow_succ],
-  rw nat.bit1_val, simp, linarith [ih],
-end
-
-lemma decode_nat_ub (l : list bool) (h : l ≠ []) : 2^(l.length - 1) ≤ decode_nat l :=
-begin
-  induction l with hd tl ih, { contradiction, }, clear h,
-  cases tl with h t, { cases hd; dec_trivial, },
-  specialize ih _, { trivial, },
-  cases hd; simp [nat.bit] at ⊢ ih,
-  { conv_rhs { rw nat.bit0_val }, rw [pow_add, mul_comm], simpa, },
-  conv_rhs { rw nat.bit1_val }, rw [pow_add, mul_comm], linarith [ih],
-end
-
-@[simp] lemma decode_nat_zero_iff_nil (l : list bool) : decode_nat l = 0 ↔ l = [] :=
-begin
-  split, swap, { rintro rfl, simp, },
-  intro h,
-  by_contra H,
-  have := decode_nat_ub l H,
-  rw [h, nonpos_iff_eq_zero] at this,
-  apply pow_ne_zero _ _ this, trivial,
-end
-
-lemma decode_nat_mono (l₁ l₂ : list bool) (hl₁ : l₁.last'.get_or_else tt = tt) (h : l₁.length < l₂.length) :
-  (decode_nat l₁) < (decode_nat l₂) :=
-begin
-  have h₁ := decode_nat_lb l₁ hl₁,
-  have h₂ := decode_nat_ub l₂ (λ z, by { subst z, simpa using h, }),
-  have : (2^l₁.length : ℤ) - 1 < 2^(l₂.length - 1),
-  { have : l₁.length ≤ l₂.length - 1,
-    { zify, rw int.coe_nat_sub,
-      { apply int.le_of_lt_add_one, simpa using h, },
-      rw nat.succ_le_iff, exact pos_of_gt h, },
-    rw int.sub_one_lt_iff, apply pow_le_pow, { norm_num, }, { assumption, }, },
-  zify at ⊢ h₂,
-  exact lt_of_lt_of_le (lt_of_le_of_lt h₁ this) h₂,
-end
-
-lemma decode_nat_quasimono (l₁ l₂ : list bool) (h : l₁.length + 1 < l₂.length) :
-  (decode_nat l₁) < (decode_nat l₂) :=
-begin
-  rcases H : l₁.last' with _|_|_,
-  { apply decode_nat_mono, { rw H, refl }, linarith only [h], },
-  { rw decode_nat_invalid l₁, apply decode_nat_mono, { simp, }, { simpa }, rw H, simp, },
-  { apply decode_nat_mono, { rw H, simp, }, linarith only [h], },
-end
-
-lemma decode_nat_tail_lt (l : list bool) (hl : l ≠ []) : decode_nat l.tail < decode_nat l :=
-begin
-  rcases H : l.last' with _|_|_,
-  { rw list.last_eq_none_iff at H, contradiction, },
-  { rw decode_nat_invalid l H, apply decode_nat_quasimono, rw ← list.length_pos_iff_ne_nil at hl, simp, nlinarith, },
-  apply decode_nat_mono,
-  rcases e : l.tail.last' with _|_|_, { refl, }, { cases option.mem_unique (list.last'_of_tail e) H, }, { refl, },
-  rw ← list.length_pos_iff_ne_nil at hl, simp, nlinarith,
-end
-
-
-end computability
+### Nat pairing
+  - `nat.mkpair'` Encodes a pair of natural numbers with logarithmic overhead i.e.
+      `log₂ (nat.mkpair a b) = log₂ a + log₂ b + O(log log a)`
+-/
 
 namespace list
 
-/-- (a, b) -> 2|a| + b size pairing function -/
+/-- A preliminary pairing function.
+This encodes (a, b) as a unary encoding of the length of `a` followed by `a ++ b`. -/
 def mkpair' (a b : list bool) : list bool :=
-(list.repeat ff a.length) ++ (tt :: (a ++ b))
+(repeat ff a.length) ++ (tt :: (a ++ b))
 
+/-- Left inverse to `list.mkpair'` -/
 def unpair' (x : list bool) : list bool × list bool :=
 (x.after (=tt)).split_at (x.take_while (=ff)).length
 
-@[simp] lemma unpair'_mkpair' (a b : list bool) :
-  unpair' (mkpair' a b) = (a, b) :=
+@[simp] lemma unpair'_mkpair' (a b : list bool) : unpair' (mkpair' a b) = (a, b) :=
 begin
-  simp only [unpair'],
   have h₁ : (mkpair' a b).after (=tt) = a ++ b,
-  { apply list.after_spec, { simp [list.mem_repeat], }, { refl, }, },
+  { apply after_spec, { simp [mem_repeat], }, { refl, }, },
   have h₂ : ((mkpair' a b).take_while (=ff)).length = a.length,
-  { erw list.take_while_spec, { apply list.length_repeat, }, { simp [list.mem_repeat], }, trivial, },
-  simp [h₁, h₂],
+  { erw take_while_spec, { apply length_repeat, }, { simp [mem_repeat], }, trivial, },
+  simp [unpair', h₁, h₂],
 end
 
+/-- Size bound for `mkpair'`: `|(a, b)| = O(|a|) + |b|` -/
 @[simp] lemma mkpair'_length (a b : list bool) : (mkpair' a b).length = 2*a.length + b.length + 1 :=
 by { simp [mkpair'], ring, }
 
+/-- The efficient pairing function on `list bool`'s.
+This function encodes (a, b) as a unary encoding of the number of bits in `a.length`, followed
+by `a.length`, followed by `a ++ b`. -/
 def mkpair (a b : list bool) : list bool :=
-mkpair' (encode_nat a.length) (a ++ b)
+mkpair' (num.to_bits a.length) (a ++ b)
 
+/-- Left inverse to `list.mkpair` -/
 def unpair (ls : list bool) : list bool × list bool :=
-(unpair' ls).2.split_at (decode_nat (unpair' ls).1)
+(unpair' ls).2.split_at (num.of_bits (unpair' ls).1)
 
-@[simp] lemma mkpair_unpair (a b : list bool) : unpair (mkpair a b) = (a, b) :=
+@[simp] lemma unpair_mkpair (a b : list bool) : unpair (mkpair a b) = (a, b) :=
 by simp [unpair, mkpair]
 
 lemma mkpair_length (a b : list bool) : (mkpair a b).length =
   if a.length = 0 then b.length + 1 else 2*(nat.log 2 a.length) + a.length + b.length + 3 :=
-begin
-  simp [mkpair, computability.encode_nat_len],
-  split_ifs with h, { rw h, ring, }, ring, 
-end
+by { split_ifs with h; simp [mkpair, num.to_bits_len, h], ring, }
 
-lemma mkpair_length_le (a b : list bool) : (mkpair a b).length ≤ 2*(nat.log 2 a.length) + a.length + b.length + 3 :=
+/-- Size bound for `mkpair'`: `|(a, b)| = |a| + |b| + O(log |a|)` -/
+lemma mkpair_length_le (a b : list bool) :
+  (mkpair a b).length ≤ 2*(nat.log 2 a.length) + a.length + b.length + 3 :=
 by { rw mkpair_length, split_ifs; linarith, }
 
-lemma mkpair'_last (a b : list bool) : (mkpair' a b).last' =
-  some (b.last'.get_or_else (a.last'.get_or_else tt)) :=
+/-- A nice coincidence in our choice of pairing function: if `a` and `b` have most significant
+bit `1`, then so does `mkpair' a b`. This allows for easy encoding of nat's in the standard way -/
+lemma mkpair_mem_num_encode_range {a b : list bool}
+  (h₁ : b ∈ set.range num.to_bits) (h₂ : b = [] → a ∈ set.range num.to_bits) :
+  a.mkpair b ∈ set.range num.to_bits :=
 begin
-  simp only [mkpair'],
-  cases b, cases a,
-  all_goals { simp [option.get_or_else_eq_get_of_some _ (list.last_cons_is_some _ _)], },
+  simp only [mkpair, mkpair', num.mem_to_bits_range_iff] at ⊢ h₁ h₂,
+  induction b using list.reverse_cases_on with st lt, swap,
+  { simpa [last'_eq_head'_reverse] using h₁, },
+  induction a using list.reverse_cases_on with st lt, swap,
+  { simpa [last'_eq_head'_reverse] using h₂, },
+  right, simp,
 end
 
-lemma mkpair_last (a b : list bool) : (mkpair a b).last' =
-  some (b.last'.get_or_else (a.last'.get_or_else tt)) :=
+lemma unpair_fst_len_lt (a : list bool) (ha : a ≠ []) : a.unpair.1.length < a.length :=
 begin
-  simp only [mkpair, mkpair'_last],
-  cases b, cases a,
-  all_goals { simp [option.get_or_else_eq_get_of_some _ (list.last_cons_is_some _ _)], },
+  simp only [unpair, unpair', drop_drop, length_drop, length_take, split_at_eq_take_drop],
+  rcases a with _|_|_, { simp at ha, contradiction, }, all_goals { clear ha },
+  { simp only [min_lt_iff], right, apply nat.lt_of_le_of_lt (nat.sub_le _ _),
+    simpa [after, nat.lt_succ_iff] using length_le_of_sublist (after_sublist _ _), },
+  { simp only [min_lt_iff], left, simp [take_while], },
 end
 
-lemma unpair'_snd_last (x : list bool) (hx : tt ∈ x.last') : (unpair' x).2.last'.get_or_else tt = tt :=
-begin
-  simp [unpair'],
-  set l := (take_while (λ a, a = ff) x).length with e, rw ← e,
-  by_cases l < (after (=tt) x).length,
-  { simp [h], have := after_last x (=tt) ff,
-    cases (after (=tt) x).last' with val, { refl, },
-    simp at this, cases val, { cases option.mem_unique hx (this rfl), },
-    refl, },
-  simp at h, simp [h],
-end
-
-lemma unpair_snd_last (x : list bool) (hx : tt ∈ x.last') : (unpair x).2.last'.get_or_else tt = tt :=
-begin
-  simp [unpair], set l := decode_nat x.unpair'.fst,
-  by_cases l < x.unpair'.snd.length,
-  { simp [h, unpair'_snd_last x hx], },
-  simp at h, simp [h],
-end
-
-lemma unpair_fst_len_lt (a : list bool) (ha : 1 < a.length) : (unpair a).1.length + 1 < a.length :=
-begin
-  simp only [unpair, unpair', list.drop_drop, list.length_drop, list.length_take, list.split_at_eq_take_drop],
-  rcases a with _|_|_, { simp at ha, contradiction, },
-  { simp only [length, add_lt_add_iff_right, min_lt_iff], right,
-    apply nat.lt_of_le_of_lt (nat.sub_le _ _),
-    simpa [after, after_length_lt] using ha, },
-  { simp only [length, add_lt_add_iff_right, min_lt_iff], left,
-    simpa [take_while, if_false] using ha, },
-end
-
-lemma unpair_snd_len_lt (a : list bool) (ha : a ≠ []) : (unpair a).2.length < a.length :=
+lemma unpair_snd_len_lt (a : list bool) (ha : a ≠ []) : a.unpair.2.length < a.length :=
 begin
   simp only [unpair, unpair', drop_drop, split_at_eq_take_drop, length_drop],
   apply lt_of_le_of_lt (nat.sub_le _ _),
@@ -345,73 +113,64 @@ end
 end list
 
 namespace nat
+open num (to_bits of_bits)
 
-def mkpair' (a b : ℕ) : ℕ := 
-decode_nat (list.mkpair (encode_nat a) (encode_nat b))
+/-- Efficient pairing function on ℕ, where result has size log(a) + log(b) + O(log log a) bits -/
+def mkpair' (a b : ℕ) : ℕ :=
+of_bits (list.mkpair (to_bits a) (to_bits b))
 
+/-- Unpairing function for `mkpair'` -/
 def unpair' (n : ℕ) : ℕ × ℕ :=
-(decode_nat (list.unpair (encode_nat n)).1, decode_nat (list.unpair (encode_nat n)).2)
-
-lemma unpair'_fst_lt (n : ℕ) : (unpair' n.succ).1 < n.succ :=
-begin
-  cases n, { dec_trivial, },
-  simp only [unpair'], conv_rhs { rw ← computability.decode_encode_nat n.succ.succ, },
-  apply computability.decode_nat_quasimono,
-  apply list.unpair_fst_len_lt,
-  simp [computability.encode_nat_len, pos_iff_ne_zero, log_eq_zero_iff, succ_eq_add_one],
-  push_neg, simp [add_assoc],
-end
-
-lemma unpair'_fst_le (n : ℕ) : (unpair' n).1 ≤ n :=
-by { cases n, dec_trivial, exact le_of_lt (unpair'_fst_lt _), }
-
-lemma unpair'_snd_lt (n : ℕ) : (unpair' n.succ).2 < n.succ :=
-begin
-  simp only [unpair'], conv_rhs { rw ← computability.decode_encode_nat n.succ, },
-  apply computability.decode_nat_mono,
-  { rw list.unpair_snd_last,
-    have := computability.encode_nat_last n.succ,
-    rw option.get_or_else_eq_get_of_some at this, swap,
-    { simpa using computability.encode_nat_succ_ne_nil n, },
-    rw ← this, exact option.get_mem _, },
-  apply list.unpair_snd_len_lt _ (computability.encode_nat_succ_ne_nil n),
-end
-
-lemma unpair'_snd_le (n : ℕ) : n.unpair'.2 ≤ n :=
-by { cases n, dec_trivial, exact le_of_lt (unpair'_snd_lt _), }
+(of_bits (list.unpair (to_bits n)).1, of_bits (list.unpair (to_bits n)).2)
 
 @[simp] lemma unpair'_mkpair' (a b : ℕ) : unpair' (mkpair' a b) = (a, b) :=
 begin
-  simp only [unpair', mkpair'],
-  rw computability.encode_decode_nat, { simp },
-  simp [list.mkpair_last],
+  simp only [unpair', mkpair', num.of_to_nat],
+  rw num.to_bits_of_bits_valid, { simp, },
+  exact list.mkpair_mem_num_encode_range (set.mem_range_self _) (λ _, set.mem_range_self _),
 end
 
 lemma mkpair'_zero (a : ℕ) : mkpair' 0 a = bit1 a :=
-by simp [mkpair', list.mkpair, list.mkpair', nat.bit]
-
-lemma mkpair'_one (a : ℕ) : mkpair' 1 a = bit0 (bit1 (bit1 (bit1 a))) :=
-by simp [mkpair', list.mkpair, list.mkpair', nat.bit]
-
-lemma mkpair'_ne_zero (a b : ℕ) : mkpair' a b ≠ 0 :=
 by simp [mkpair', list.mkpair, list.mkpair']
 
-lemma mkpair'_le (a b : ℕ) : nat.log 2 (mkpair' a b) ≤
-  log 2 a + log 2 b + 2 * log 2 (log 2 a + 1) + 5 :=
+lemma mkpair'_one (a : ℕ) : mkpair' 1 a = bit0 (bit1 (bit1 (bit1 a))) :=
+by { simp [mkpair', list.mkpair, list.mkpair', to_bits, (show 1 = num.pos 1, from rfl)], }
+
+lemma mkpair'_ne_zero (a b : ℕ) : mkpair' a b ≠ 0 :=
+by { simp only [mkpair', list.mkpair, list.mkpair'], norm_cast, simp, }
+
+lemma unpair'_fst_lt (n : ℕ) : (unpair' n.succ).1 < n.succ :=
 begin
-  simp only [mkpair'],
-  exact calc log 2 (decode_nat (list.mkpair (encode_nat a) (encode_nat b)))
-        ≤ log 2 (2^((list.mkpair (encode_nat a) (encode_nat b)).length) - 1) :
-          by { apply log_monotone, zify [int.coe_nat_sub (one_le_iff_ne_zero.mpr (pow_ne_zero _ (show 2 ≠ 0, by norm_num)))], 
-               apply computability.decode_nat_lb, rw list.mkpair_last, simp, }
-    ...  ≤ (list.mkpair (encode_nat a) (encode_nat b)).length :
-          by { conv_rhs { rw ← log_pow (show 1 < 2, by norm_num) (list.mkpair _ _).length }, apply log_monotone, exact tsub_le_self, }
-    ... ≤ 2*(log 2 (encode_nat a).length) + (encode_nat a).length + (encode_nat b).length + 3 : list.mkpair_length_le _ _
-    ... ≤ 2*(log 2 (log 2 a + 1)) + (log 2 a + 1) + (log 2 b + 1) + 3 :
-          by { mono*, all_goals { try { apply log_monotone}, try { exact zero_le _, }, }, all_goals { exact computability.encode_nat_len_le _, }, }
-    ... = _ : by ring_nf
+  convert_to (unpair' n.succ).1 < of_bits (to_bits n.succ), { simp, },
+  apply num.of_bits_strict_mono,
+  apply list.unpair_fst_len_lt, simp, norm_cast, simp,
 end
 
+lemma unpair'_fst_le (n : ℕ) : (unpair' n).1 ≤ n := by { cases n, { refl, }, exact le_of_lt (unpair'_fst_lt _), }
+
+lemma unpair'_snd_lt (n : ℕ) : (unpair' n.succ).2 < n.succ :=
+begin
+  convert_to (unpair' n.succ).2 < of_bits (to_bits n.succ), { simp, },
+  apply num.of_bits_strict_mono,
+  apply list.unpair_snd_len_lt, simp, norm_cast, simp,
+end
+
+lemma unpair'_snd_le (n : ℕ) : (unpair' n).2 ≤ n := by { cases n, { refl, }, exact le_of_lt (unpair'_snd_lt _), }
+
+/-- Size bound for `mkpair'`: `log₂ (mkpair' a b) = log₂ a + log₂ b + O(log log a) `-/
+lemma mkpair'_le (a b : ℕ) : log 2 (mkpair' a b) ≤
+  log 2 a + log 2 b + 2 * log 2 (log 2 a + 1) + 5 :=
+calc log 2 (of_bits (list.mkpair (to_bits a) (to_bits b)))
+    ≤ log 2 (2^((list.mkpair (to_bits a) (to_bits b)).length) - 1) :
+      by { apply log_monotone, apply le_pred_of_lt, apply num.of_bits_lt, }
+... ≤ (list.mkpair (to_bits a) (to_bits b)).length :
+      by { conv_rhs { rw ← log_pow (show 1 < 2, by norm_num) (list.mkpair _ _).length },
+           apply log_monotone, exact tsub_le_self, }
+... ≤ 2*(log 2 (to_bits a).length) + (to_bits a).length + (to_bits b).length + 3 :
+      list.mkpair_length_le _ _
+... ≤ 2*(log 2 (log 2 a + 1)) + (log 2 a + 1) + (log 2 b + 1) + 3 :
+      by { mono*, all_goals { try { apply log_monotone }, try { exact zero_le _, }, },
+           all_goals { convert num.to_bits_len_le _, simp, }, }
+... = _ : by ring_nf
+
 end nat
-
-
